Integrated several addition laws for parallel composition and iteration

theories/sf_rdes/utp_sfrd_healths.thy
@@ -548,6 +548,9 @@ lemma NCSP_preR_CRC [closure]:
   shows "pre\<^sub>R(P) is CRC"
   by (rule CRC_intro, simp_all add: closure assms unrest)
 
+lemma NCSP_postR_CRF [closure]: "P is NCSP \<Longrightarrow> post\<^sub>R P is CRF"
+  by (rule CRF_intro, simp_all add: unrest closure)
+
 lemma CSP3_Sup_closure [closure]:
   "A \<subseteq> \<lbrakk>CSP3\<rbrakk>\<^sub>H \<Longrightarrow> (\<Sqinter> A) is CSP3"
   apply (auto simp add: CSP3_def Healthy_def seq_Sup_distl)
@@ -683,19 +686,23 @@ qed (simp_all)
 abbreviation TestC ("test\<^sub>C") where
 "test\<^sub>C P \<equiv> csp_theory.utp_test P"
 
-abbreviation StarC :: "('\<sigma>, '\<phi>) action \<Rightarrow> ('\<sigma>, '\<phi>) action" ("_\<^sup>\<star>\<^sup>C" [999] 999) where
+definition StarC :: "('\<sigma>, '\<phi>) action \<Rightarrow> ('\<sigma>, '\<phi>) action" ("_\<^sup>\<star>\<^sup>C" [999] 999) where
 "StarC P \<equiv> csp_theory.utp_star P"
 
 lemma sfrd_star_as_rdes_star:
-  "P is NCSP \<Longrightarrow> P\<^sup>\<star>\<^sup>C = P\<^sup>\<star>\<^sup>R ;; Skip"
-  by (simp add: csp_theory.Star_alt_def nsrdes_theory.Star_alt_def StarR_def closure unrest Skip_srdes_left_unit csp_theory.Unit_Right)
+  "P is NCSP \<Longrightarrow> P\<^sup>\<star>\<^sup>R ;; Skip = P\<^sup>\<star>\<^sup>C"
+  by (simp add: csp_theory.Star_alt_def nsrdes_theory.Star_alt_def StarC_def StarR_def closure unrest Skip_srdes_left_unit csp_theory.Unit_Right)
+
+lemma sfrd_star_as_rdes_star':
+  "P is NCSP \<Longrightarrow> Skip ;; P\<^sup>\<star>\<^sup>R = P\<^sup>\<star>\<^sup>C"
+  by (simp add: csp_theory.Star_alt_def nsrdes_theory.Star_alt_def StarC_def StarR_def closure unrest Skip_srdes_right_unit csp_theory.Unit_Left upred_semiring.distrib_left)
 
 theorem csp_star_rdes_def [rdes_def]:
   assumes "P is CRC" "Q is CRR" "R is CRF" "$st\<acute> \<sharp> Q"
   shows "(\<^bold>R\<^sub>s(P \<turnstile> Q \<diamondop> R))\<^sup>\<star>\<^sup>C = \<^bold>R\<^sub>s(R\<^sup>\<star>\<^sup>c wp\<^sub>r P \<turnstile> (R\<^sup>\<star>\<^sup>c ;; Q) \<diamondop> R\<^sup>\<star>\<^sup>c)"
-  apply (simp add: wp_rea_def sfrd_star_as_rdes_star crf_star_as_rea_star assms seqr_assoc rpred closure unrest StarR_rdes_def)
+  apply (simp add: wp_rea_def sfrd_star_as_rdes_star[THEN sym] crf_star_as_rea_star assms seqr_assoc rpred closure unrest StarR_rdes_def)
   apply (simp add: rdes_def assms closure unrest wp_rea_def[THEN sym])
-  apply (simp add: wp  rpred assms closure)
+  apply (simp add: wp rpred assms closure)
   apply (simp add: csp_do_nothing) 
   done
 
